+++
title = '2.3 Examples'
weight = 2
+++

## 2.3 Product Rule: Examples

#### Ex1.

Differentiate \( f(x) = x^3 \cdot (4x - 2) \)

**Solution**:

We define \( u(x) = x^3 \) and \( v(x) = 4x - 2 \).

1. Differentiate \( u(x) = x^3 \):  
   \( u'(x) = 3x^2 \)

2. Differentiate \( v(x) = 4x - 2 \):  
   \( v'(x) = 4 \)

Now apply the product rule:

\[
f'(x) = u'(x) \cdot v(x) + u(x) \cdot v'(x)
\]

\[
f'(x) = (3x^2) \cdot (4x - 2) + (x^3) \cdot 4
\]

Simplifying:

\[
f'(x) = 12x^3 - 6x^2 + 4x^3
\]

\[
f'(x) = 16x^3 - 6x^2
\]

Thus, the derivative is:

\[
f'(x) = 16x^3 - 6x^2
\]

---

#### Ex2.

Differentiate \( f(x) = (5x^2 + 3x) \cdot (x^4 - 2x) \)

**Solution**:

We define \( u(x) = 5x^2 + 3x \) and \( v(x) = x^4 - 2x \).

1. Differentiate \( u(x) = 5x^2 + 3x \):  
   \( u'(x) = 10x + 3 \)

2. Differentiate \( v(x) = x^4 - 2x \):  
   \( v'(x) = 4x^3 - 2 \)

Now apply the product rule:

\[
f'(x) = u'(x) \cdot v(x) + u(x) \cdot v'(x)
\]

\[
f'(x) = (10x + 3) \cdot (x^4 - 2x) + (5x^2 + 3x) \cdot (4x^3 - 2)
\]

Simplifying:

\[
f'(x) = (10x + 3)(x^4 - 2x) + (5x^2 + 3x)(4x^3 - 2)
\]

Expanding both terms:

\[
f'(x) = 10x(x^4 - 2x) + 3(x^4 - 2x) + 5x^2(4x^3 - 2) + 3x(4x^3 - 2)
\]

Simplifying each term:

\[
f'(x) = 10x^5 - 20x^2 + 3x^4 - 6x + 20x^5 - 10x^2 + 12x^4 - 6x
\]

Combining like terms:

\[
f'(x) = 30x^5 + 15x^4 - 30x^2 - 12x
\]

Thus, the derivative is:

\[
f'(x) = 30x^5 + 15x^4 - 30x^2 - 12x
\]

---

#### Ex3.

Differentiate \( f(x) = \frac{1}{x} \cdot (3x^2 + 2x) \)

**Solution**:

We define \( u(x) = \frac{1}{x} \) and \( v(x) = 3x^2 + 2x \).

1. Differentiate \( u(x) = \frac{1}{x} \):  
   \( u'(x) = -\frac{1}{x^2} \)

2. Differentiate \( v(x) = 3x^2 + 2x \):  
   \( v'(x) = 6x + 2 \)

Now apply the product rule:

\[
f'(x) = u'(x) \cdot v(x) + u(x) \cdot v'(x)
\]

\[
f'(x) = \left(-\frac{1}{x^2}\right) \cdot (3x^2 + 2x) + \left(\frac{1}{x}\right) \cdot (6x + 2)
\]

Simplifying:

\[
f'(x) = -\frac{3x^2 + 2x}{x^2} + \frac{6x + 2}{x}
\]

\[
f'(x) = -\frac{3}{x} - \frac{2}{x^2} + \frac{6}{x} + \frac{2}{x}
\]

Combining like terms:

\[
f'(x) = \frac{5}{x} - \frac{2}{x^2}
\]

Thus, the derivative is:

\[
f'(x) = \frac{5}{x} - \frac{2}{x^2}
\]

---

#### Ex4.

Differentiate \( f(x) = (x^2 - 4) \cdot (x + 1) \)

**Solution**:

We define \( u(x) = x^2 - 4 \) and \( v(x) = x + 1 \).

1. Differentiate \( u(x) = x^2 - 4 \):  
   \( u'(x) = 2x \)

2. Differentiate \( v(x) = x + 1 \):  
   \( v'(x) = 1 \)

Now apply the product rule:

\[
f'(x) = u'(x) \cdot v(x) + u(x) \cdot v'(x)
\]

\[
f'(x) = (2x) \cdot (x + 1) + (x^2 - 4) \cdot 1
\]

Simplifying:

\[
f'(x) = 2x(x + 1) + (x^2 - 4)
\]

\[
f'(x) = 2x^2 + 2x + x^2 - 4
\]

Combining like terms:

\[
f'(x) = 3x^2 + 2x - 4
\]

Thus, the derivative is:

\[
f'(x) = 3x^2 + 2x - 4
\]

---

#### Ex5.

Differentiate \( f(x) = (x + 1) \cdot \frac{1}{x} \)

**Solution**:

We define \( u(x) = x + 1 \) and \( v(x) = \frac{1}{x} \).

1. Differentiate \( u(x) = x + 1 \):  
   \( u'(x) = 1 \)

2. Differentiate \( v(x) = \frac{1}{x} \):  
   \( v'(x) = -\frac{1}{x^2} \)

Now apply the product rule:

\[
f'(x) = u'(x) \cdot v(x) + u(x) \cdot v'(x)
\]

\[
f'(x) = (1) \cdot \frac{1}{x} + (x + 1) \cdot \left(-\frac{1}{x^2}\right)
\]

Simplifying:

\[
f'(x) = \frac{1}{x} - \frac{x + 1}{x^2}
\]

\[
f'(x) = \frac{1}{x} - \frac{x}{x^2} - \frac{1}{x^2}
\]

\[
f'(x) = \frac{1}{x} - \frac{1}{x} - \frac{1}{x^2}
\]

\[
f'(x) = -\frac{1}{x^2}
\]

Thus, the derivative is:

\[
f'(x) = -\frac{1}{x^2}
\]

---
