+++
title = '2.3 Practice'
weight = 2
+++

## 2.3 Product Rule: Practice

#### Ex1.

Differentiate \( f(x) = (x^2 + 3x) \cdot (x^3 - 5) \)

<details>
  <summary>
    <strong id="solution-title">Solution</strong>
  </summary>

We define \( u(x) = x^2 + 3x \) and \( v(x) = x^3 - 5 \).

1. Differentiate \( u(x) = x^2 + 3x \):  
   \( u'(x) = 2x + 3 \)

2. Differentiate \( v(x) = x^3 - 5 \):  
   \( v'(x) = 3x^2 \)

Now apply the product rule:

\[
f'(x) = u'(x) \cdot v(x) + u(x) \cdot v'(x)
\]

\[
f'(x) = (2x + 3) \cdot (x^3 - 5) + (x^2 + 3x) \cdot (3x^2)
\]

Simplifying:

\[
f'(x) = (2x + 3)(x^3 - 5) + (x^2 + 3x)(3x^2)
\]

Expanding each term:

\[
f'(x) = 2x(x^3 - 5) + 3(x^3 - 5) + 3x^2(x^2 + 3x)
\]

Simplifying further:

\[
f'(x) = 2x^4 - 10x + 3x^3 - 15 + 3x^4 + 9x^3
\]

Combining like terms:

\[
f'(x) = 5x^4 + 12x^3 - 10x - 15
\]

Thus, the derivative is:

\[
f'(x) = 5x^4 + 12x^3 - 10x - 15
\]

</details>

---

#### Ex2.

Differentiate \( f(x) = x \cdot \sqrt{x^3} \)

<details>
  <summary>
    <strong id="solution-title">Solution</strong>
  </summary>

We define \( u(x) = x \) and \( v(x) = x^{3/2} \).

1. Differentiate \( u(x) = x \):  
   \( u'(x) = 1 \)

2. Differentiate \( v(x) = x^{3/2} \):  
   Use the power rule:  
   \( v'(x) = \frac{3}{2} x^{1/2} \)

Now apply the product rule:

\[
f'(x) = u'(x) \cdot v(x) + u(x) \cdot v'(x)
\]

\[
f'(x) = 1 \cdot x^{3/2}  + x \cdot \frac{3}{2} x^{1/2} 
\]

Simplifying:

\[
f'(x) = x^{3/2}  + \frac{3}{2} x^{3/2} 
\]

Thus, the derivative is:

\[
f'(x) = \frac{5}{2} x^{3/2} 
\]

</details>

---

#### Ex3.

Differentiate \( f(x) = (3x - 2) \cdot (x^2 + 4) \)

<details>
  <summary>
    <strong id="solution-title">Solution</strong>
  </summary>

We define \( u(x) = 3x - 2 \) and \( v(x) = x^2 + 4 \).

1. Differentiate \( u(x) = 3x - 2 \):  
   \( u'(x) = 3 \)

2. Differentiate \( v(x) = x^2 + 4 \):  
   \( v'(x) = 2x \)

Now apply the product rule:

\[
f'(x) = u'(x) \cdot v(x) + u(x) \cdot v'(x)
\]

\[
f'(x) = 3 \cdot (x^2 + 4) + (3x - 2) \cdot 2x
\]

Simplifying:

\[
f'(x) = 3x^2 + 12 + 6x^2 - 4x
\]

Combining like terms:

\[
f'(x) = 9x^2 - 4x + 12
\]

Thus, the derivative is:

\[
f'(x) = 9x^2 - 4x + 12
\]

</details>

---

#### Ex4.

Differentiate \( f(x) = x^3 \cdot \sqrt{x} \)

<details>
  <summary>
    <strong id="solution-title">Solution</strong>
  </summary>

We define \( u(x) = x^3 \) and \( v(x) = \sqrt{x} = x^{1/2} \).

1. Differentiate \( u(x) = x^3 \):  
   \( u'(x) = 3x^2 \)

2. Differentiate \( v(x) = x^{1/2} \):  
   \( v'(x) = \frac{1}{2} x^{-1/2} \)

Now apply the product rule:

\[
f'(x) = u'(x) \cdot v(x) + u(x) \cdot v'(x)
\]

\[
f'(x) = (3x^2) \cdot x^{1/2} + x^3 \cdot \frac{1}{2} x^{-1/2}
\]

Simplifying:

\[
f'(x) = 3x^{5/2} + \frac{1}{2} x^{5/2}
\]

Combining like terms:

\[
f'(x) = \frac{7}{2} x^{5/2}
\]

Thus, the derivative is:

\[
f'(x) = \frac{7}{2} x^{5/2}
\]

</details>

---

#### Ex5.

Differentiate \( f(x) = (x^2 + 1) \cdot (x^3 - 3x) \)

<details>
  <summary>
    <strong id="solution-title">Solution</strong>
  </summary>

We define \( u(x) = x^2 + 1 \) and \( v(x) = x^3 - 3x \).

1. Differentiate \( u(x) = x^2 + 1 \):  
   \( u'(x) = 2x \)

2. Differentiate \( v(x) = x^3 - 3x \):  
   \( v'(x) = 3x^2 - 3 \)

Now apply the product rule:

\[
f'(x) = u'(x) \cdot v(x) + u(x) \cdot v'(x)
\]

\[
f'(x) = (2x) \cdot (x^3 - 3x) + (x^2 + 1) \cdot (3x^2 - 3)
\]

Expanding:

\[
f'(x) = 2x(x^3 - 3x) + (x^2 + 1)(3x^2 - 3)
\]

Simplifying:

\[
f'(x) = 2x^4 - 6x^2 + 3x^4 - 3x^2 + 3x^2 - 3
\]

Combining like terms:

\[
f'(x) = 5x^4 - 6x^2 - 3
\]

Thus, the derivative is:

\[
f'(x) = 5x^4 - 6x^2 - 3
\]

</details>

---

<iframe src="https://script.google.com/macros/s/AKfycbx3eZ8cj_W2S3gPRQnlc4Y8x84nUF4GKa4yUM8g7RvoL9AUqU5bnho562Rr9szNjemX/exec" width="100%" height="1000px" frameborder="0" marginheight="0" marginwidth="0">Loading...</iframe>

