+++
title = '2.2 Examples'
weight = 2
+++

### 2.2 Sum and Difference Rules

#### Ex1.

Differentiate the function \( f(x) = x^4 + 2x^3 - 5x + 7 \).

**Solution:**

Using the Sum Rule, differentiate each term:

\[
f'(x) = \frac{d}{dx}[x^4] + \frac{d}{dx}[2x^3] - \frac{d}{dx}[5x] + \frac{d}{dx}[7]
\]

\[
f'(x) = 4x^3 + 6x^2 - 5
\]

Thus, the derivative of \( f(x) = x^4 + 2x^3 - 5x + 7 \) is:

\[
f'(x) = 4x^3 + 6x^2 - 5
\]

---

#### Ex2.

Differentiate the function \( f(x) = 3x^5 - 2x^4 + x^3 - 6 \).

**Solution:**

Using the Sum and Difference Rules, differentiate each term:

\[
f'(x) = \frac{d}{dx}[3x^5] - \frac{d}{dx}[2x^4] + \frac{d}{dx}[x^3] - \frac{d}{dx}[6]
\]

\[
f'(x) = 15x^4 - 8x^3 + 3x^2
\]

Thus, the derivative of \( f(x) = 3x^5 - 2x^4 + x^3 - 6 \) is:

\[
f'(x) = 15x^4 - 8x^3 + 3x^2
\]

---

#### Ex3.

Differentiate the function \( f(x) = x^3 - 4x^2 + 9x - 2 \).

**Solution:**

Using the Sum Rule, differentiate each term:

\[
f'(x) = \frac{d}{dx}[x^3] - \frac{d}{dx}[4x^2] + \frac{d}{dx}[9x] - \frac{d}{dx}[2]
\]

\[
f'(x) = 3x^2 - 8x + 9
\]

Thus, the derivative of \( f(x) = x^3 - 4x^2 + 9x - 2 \) is:

\[
f'(x) = 3x^2 - 8x + 9
\]

---

#### Ex4.

Differentiate the function \( f(x) = -7x^6 + 5x^4 - 2x^3 \).

**Solution:**

Using the Sum and Difference Rules, differentiate each term:

\[
f'(x) = \frac{d}{dx}[-7x^6] + \frac{d}{dx}[5x^4] - \frac{d}{dx}[2x^3]
\]

\[
f'(x) = -42x^5 + 20x^3 - 6x^2
\]

Thus, the derivative of \( f(x) = -7x^6 + 5x^4 - 2x^3 \) is:

\[
f'(x) = -42x^5 + 20x^3 - 6x^2
\]

---

#### Ex5.

Differentiate the function \( f(x) = \frac{1}{4}x^3 - 2x + 5 \).

**Solution:**

Using the Sum and Difference Rules, differentiate each term:

\[
f'(x) = \frac{d}{dx}[\frac{1}{4}x^3] - \frac{d}{dx}[2x] + \frac{d}{dx}[5]
\]

\[
f'(x) = \frac{3}{4}x^2 - 2
\]

Thus, the derivative of \( f(x) = \frac{1}{4}x^3 - 2x + 5 \) is:

\[
f'(x) = \frac{3}{4}x^2 - 2
\]

---

#### Ex6.

Differentiate the function \( f(x) = 2x^7 - x^5 + 4x^2 \).

**Solution:**

Using the Sum and Difference Rules, differentiate each term:

\[
f'(x) = \frac{d}{dx}[2x^7] - \frac{d}{dx}[x^5] + \frac{d}{dx}[4x^2]
\]

\[
f'(x) = 14x^6 - 5x^4 + 8x
\]

Thus, the derivative of \( f(x) = 2x^7 - x^5 + 4x^2 \) is:

\[
f'(x) = 14x^6 - 5x^4 + 8x
\]

---

#### Ex7.

Differentiate the function \( f(x) = 3x^4 - 2x^2 + 6 \).

**Solution:**

Using the Sum and Difference Rules, differentiate each term:

\[
f'(x) = \frac{d}{dx}[3x^4] - \frac{d}{dx}[2x^2] + \frac{d}{dx}[6]
\]

\[
f'(x) = 12x^3 - 4x
\]

Thus, the derivative of \( f(x) = 3x^4 - 2x^2 + 6 \) is:

\[
f'(x) = 12x^3 - 4x
\]

---

#### Ex8.

Differentiate the function \( f(x) = -5x^3 + 4x^2 - x + 2 \).

**Solution:**

Using the Sum and Difference Rules, differentiate each term:

\[
f'(x) = \frac{d}{dx}[-5x^3] + \frac{d}{dx}[4x^2] - \frac{d}{dx}[x] + \frac{d}{dx}[2]
\]

\[
f'(x) = -15x^2 + 8x - 1
\]

Thus, the derivative of \( f(x) = -5x^3 + 4x^2 - x + 2 \) is:

\[
f'(x) = -15x^2 + 8x - 1
\]

---