+++
title = '2.2 Practice'
weight = 2
+++

### 2.2 Sum and Difference Rules

#### Ex1.

Differentiate the function \( f(x) = x^3 + 5x^2 - 7x + 3 \).

<details>
  <summary>
    <strong id="solution-title">Solution</strong>
  </summary>

Using the Sum Rule, differentiate each term individually:

\[
f'(x) = \frac{d}{dx}[x^3] + \frac{d}{dx}[5x^2] - \frac{d}{dx}[7x] + \frac{d}{dx}[3]
\]

\[
f'(x) = 3x^2 + 10x - 7
\]

Thus, the derivative of \( f(x) = x^3 + 5x^2 - 7x + 3 \) is:

\[
f'(x) = 3x^2 + 10x - 7
\]

</details>

---

#### Ex2.

Differentiate the function \( f(x) = 4x^2 - 9x + 6 \).

<details>
  <summary>
    <strong id="solution-title">Solution</strong>
  </summary>

Using the Sum and Difference Rules, differentiate each term:

\[
f'(x) = \frac{d}{dx}[4x^2] - \frac{d}{dx}[9x] + \frac{d}{dx}[6]
\]

\[
f'(x) = 8x - 9
\]

Thus, the derivative of \( f(x) = 4x^2 - 9x + 6 \) is:

\[
f'(x) = 8x - 9
\]

</details>

#### Ex3.

Differentiate the function \( f(x) = 3x^4 - x^2 + 2x - 5 \).

<details>
  <summary>
    <strong id="solution-title">Solution</strong>
  </summary>

Using the Sum Rule, differentiate each term:

\[
f'(x) = \frac{d}{dx}[3x^4] - \frac{d}{dx}[x^2] + \frac{d}{dx}[2x] - \frac{d}{dx}[5]
\]

\[
f'(x) = 12x^3 - 2x + 2
\]

Thus, the derivative of \( f(x) = 3x^4 - x^2 + 2x - 5 \) is:

\[
f'(x) = 12x^3 - 2x + 2
\]

</details>

---

#### Ex4.

Differentiate the function \( f(x) = x^5 - 3x^3 + 2x - 1 \).

<details>
  <summary>
    <strong id="solution-title">Solution</strong>
  </summary>

Using the Sum Rule, differentiate each term:

\[
f'(x) = \frac{d}{dx}[x^5] - \frac{d}{dx}[3x^3] + \frac{d}{dx}[2x] - \frac{d}{dx}[1]
\]

\[
f'(x) = 5x^4 - 9x^2 + 2
\]

Thus, the derivative of \( f(x) = x^5 - 3x^3 + 2x - 1 \) is:

\[
f'(x) = 5x^4 - 9x^2 + 2
\]

</details>

---

#### Ex5.

Differentiate the function \( f(x) = \frac{1}{2}x^2 - 4x + 7 \).

<details>
  <summary>
    <strong id="solution-title">Solution</strong>
  </summary>

Using the Sum and Difference Rules, differentiate each term:

\[
f'(x) = \frac{d}{dx}\left[\frac{1}{2}x^2\right] - \frac{d}{dx}[4x] + \frac{d}{dx}[7]
\]

\[
f'(x) = x - 4
\]

Thus, the derivative of \( f(x) = \frac{1}{2}x^2 - 4x + 7 \) is:

\[
f'(x) = x - 4
\]

</details>

---

#### Ex6.

Differentiate the function \( f(x) = 2x^3 - 5x + 4 \).

<details>
  <summary>
    <strong id="solution-title">Solution</strong>
  </summary>

Using the Sum and Difference Rules, differentiate each term:

\[
f'(x) = \frac{d}{dx}[2x^3] - \frac{d}{dx}[5x] + \frac{d}{dx}[4]
\]

\[
f'(x) = 6x^2 - 5
\]

Thus, the derivative of \( f(x) = 2x^3 - 5x + 4 \) is:

\[
f'(x) = 6x^2 - 5
\]

</details>

---

<iframe src="https://script.google.com/macros/s/AKfycby68F1DjkgDxseMX5uqS7QDJV7W3OqyJQPG0Fb4XYL40YLAemdebjKN8Y3ccf9LS_eRnQ/exec" width="100%" height="1000px" frameborder="0" marginheight="0" marginwidth="0">Loading...</iframe>
