+++
title = '1.1 Examples'
weight = 1
+++

## Average Rate of Change given an Equation.

### Example 1: 

Find the average rate of change of the function \(f(x) = x^2 - 2x + 1\) between \(x = 1\) and \(x = 3\).

1. Calculate \(f(1)\):
   

\[
   f(1) = 1^2 - 2(1) + 1 = 0
   \]



2. Calculate \(f(3)\):
   

\[
   f(3) = 3^2 - 2(3) + 1 = 4
   \]



3. Use the average rate of change formula:
   

\[
   \text{Average Rate of Change} = \frac{f(3) - f(1)}{3 - 1} = \frac{4 - 0}{3 - 1} = 2
   \]



So, the average rate of change of the function \(f(x) = x^2 - 2x + 1\) between \(x = 1\) and \(x = 3\) is 2.

### Example 2: 

Determine the Average Rate of Change for \(g(x) = 2x^2 + 3x - 5\) between \(x = -1\) and \(x = 2\).

1. Calculate \(g(-1)\):
   

\[
   g(-1) = 2(-1)^2 + 3(-1) - 5 = 2 - 3 - 5 = -6
\]



2. Calculate \(g(2)\):
   

\[
   g(2) = 2(2)^2 + 3(2) - 5 = 8 + 6 - 5 = 9
\]



3. Use the average rate of change formula:
   

\[
   \text{Average Rate of Change} = \frac{g(2) - g(-1)}{2 - (-1)} = \frac{9 - (-6)}{2 - (-1)} = \frac{9 + 6}{2 + 1} = \frac{15}{3} = 5
   \]



So, the average rate of change of the function \(g(x) = 2x^2 + 3x - 5\) between \(x = -1\) and \(x = 2\) is 5.




## Average Rate of Change from a Graph
### Example 3:
Let's determine the average rate of change for a function by reading points from the graph. 

![Graph of Function 1](/images/MCV4U1_1ex3.png)

1. Identify two points on the graph:
   - Point A: \( (1, 3) \)
   - Point B: \( (4, 7) \)

2. Use the average rate of change formula:
   

\[
   \text{Average Rate of Change} = \frac{f(4) - f(1)}{4 - 1} = \frac{7 - 3}{4 - 1} = \frac{4}{3} \approx 1.33
   \]



So, the average rate of change of the function between \( x = 1 \) and \( x = 4 \) is approximately 1.33.

### Example 4: Average Rate of Change from a Graph

Let's determine the average rate of change for another function by reading points from the graph. 

![Graph of Function 2](/images/MCV4U1_1ex4.png)

1. Identify two points on the graph:
   - Point C: \( (-2, 4) \)
   - Point D: \( (2, -12) \)

2. Use the average rate of change formula:
   

\[
   \text{Average Rate of Change} = \frac{f(2) - f(-2)}{2 - (-2)} = \frac{-12 - 4}{2 - (-2)} = \frac{-16}{4} = -4
   \]



So, the average rate of change of the function between \( x = -2 \) and \( x = 2 \) is -4.
