+++
title = '2.4 Examples:'
weight = 2
+++

### Example 1: Simple Rational Function

Differentiate the following function using the quotient rule:

\[
f(x) = \frac{x^2 + 2x}{x + 1}
\]

**Solution:**

- Let \( u(x) = x^2 + 2x \) and \( v(x) = x + 1 \).
- The derivatives are:
  - \( u'(x) = 2x + 2 \)
  - \( v'(x) = 1 \)

Applying the quotient rule:

\[
f'(x) = \frac{(x + 1)(2x + 2) - (x^2 + 2x)(1)}{(x + 1)^2}
\]

Now, simplify the numerator:

\[
f'(x) = \frac{(x + 1)(2x + 2) - (x^2 + 2x)}{(x + 1)^2}
\]
\[
f'(x) = \frac{2x^2 + 2x + 2x + 2 - x^2 - 2x}{(x + 1)^2}
\]
\[
f'(x) = \frac{x^2 + 2}{(x + 1)^2}
\]

Thus, the derivative is:

\[
f'(x) = \frac{x^2 + 2}{(x + 1)^2}
\]

---

### Example 2: Rational Function with a Quadratic Numerator

Differentiate the following function:

\[
f(x) = \frac{x^3 - 4x}{x^2 + 1}
\]

**Solution:**

- Let \( u(x) = x^3 - 4x \) and \( v(x) = x^2 + 1 \).
- The derivatives are:
  - \( u'(x) = 3x^2 - 4 \)
  - \( v'(x) = 2x \)

Applying the quotient rule:

\[
f'(x) = \frac{(x^2 + 1)(3x^2 - 4) - (x^3 - 4x)(2x)}{(x^2 + 1)^2}
\]

Now, expand the numerator:

\[
f'(x) = \frac{(x^2 + 1)(3x^2 - 4) - 2x(x^3 - 4x)}{(x^2 + 1)^2}
\]
\[
f'(x) = \frac{3x^4 - 4x^2 + 3x^2 - 4 - 2x^4 + 8x^2}{(x^2 + 1)^2}
\]
\[
f'(x) = \frac{x^4 + 7x^2 - 4}{(x^2 + 1)^2}
\]

Thus, the derivative is:

\[
f'(x) = \frac{x^4 + 7x^2 - 4}{(x^2 + 1)^2}
\]

---

### Example 3: Rational Function with Negative Exponent

Differentiate the following function:

\[
f(x) = \frac{5}{x^2 + 1}
\]

**Solution:**

- Let \( u(x) = 5 \) and \( v(x) = x^2 + 1 \).
- The derivatives are:
  - \( u'(x) = 0 \)
  - \( v'(x) = 2x \)

Applying the quotient rule:

\[
f'(x) = \frac{(x^2 + 1)(0) - (5)(2x)}{(x^2 + 1)^2}
\]

Simplifying:

\[
f'(x) = \frac{-10x}{(x^2 + 1)^2}
\]

Thus, the derivative is:

\[
f'(x) = \frac{-10x}{(x^2 + 1)^2}
\]

---

### Example 4: Rational Function with a Root in the Numerator

Differentiate the following function:

\[
f(x) = \frac{\sqrt{x}}{x + 2}
\]

**Solution:**

- Let \( u(x) = \sqrt{x} = x^{1/2} \) and \( v(x) = x + 2 \).
- The derivatives are:
  - \( u'(x) = \frac{1}{2}x^{-1/2} \)
  - \( v'(x) = 1 \)

Applying the quotient rule:

\[
f'(x) = \frac{(x + 2)\left(\frac{1}{2}x^{-1/2}\right) - \sqrt{x}(1)}{(x + 2)^2}
\]

Now, simplify the numerator:

\[
f'(x) = \frac{\frac{1}{2}(x + 2)x^{-1/2} - x^{1/2}}{(x + 2)^2}
\]
\[
f'(x) = \frac{\frac{x + 2}{2x^{1/2}} - x^{1/2}}{(x + 2)^2}
\]

Thus, the derivative is:

\[
f'(x) = \frac{\frac{x + 2}{2\sqrt{x}} - \sqrt{x}}{(x + 2)^2}
\]

---

### Example 5: Rational Function with a Negative Exponent

Differentiate the following function:

\[
f(x) = \frac{3}{x^{-2} + 4}
\]

**Solution:**

- Let \( u(x) = 3 \) and \( v(x) = x^{-2} + 4 \).
- The derivatives are:
  - \( u'(x) = 0 \)
  - \( v'(x) = -2x^{-3} \)

Applying the quotient rule:

\[
f'(x) = \frac{(x^{-2} + 4)(0) - (3)(-2x^{-3})}{(x^{-2} + 4)^2}
\]

Simplifying:

\[
f'(x) = \frac{6x^{-3}}{(x^{-2} + 4)^2}
\]

Thus, the derivative is:

\[
f'(x) = \frac{6x^{-3}}{(x^{-2} + 4)^2}
\]

---