+++
title = "2.5 Practice:"
weight = 2
+++

## Chain Rule:

#### Ex1. 

Differentiate the following function using the Chain Rule:

\[
y = (3x^2 + 4x + 5)^7
\]

<details>
  <summary>
    <strong id="solution-title">Solution</strong>
  </summary>

**Solution:**

1. Identify the outer and inner functions:
   - Outer function: \( u(v) = v^7 \), where \( v = 3x^2 + 4x + 5 \).
   - Inner function: \( v(x) = 3x^2 + 4x + 5 \).

2. Differentiate the outer function with respect to \( v \):
   \[
   \frac{du}{dv} = 7v^6
   \]

3. Differentiate the inner function with respect to \( x \):
   \[
   \frac{dv}{dx} = 6x + 4
   \]

4. Multiply the derivatives:
   \[
   \frac{dy}{dx} = 7(3x^2 + 4x + 5)^6 \cdot (6x + 4)
   \]

Thus, the derivative is:

\[
\frac{dy}{dx} = 7(3x^2 + 4x + 5)^6 (6x + 4)
\]

</details>

---

#### Ex2. 

Differentiate the following function using the Chain Rule:

\[
y = \sqrt{4x^3 + 5x^2 - x + 6}
\]

<details>
  <summary>
    <strong id="solution-title">Solution</strong>
  </summary>

**Solution:**

1. Rewrite the function as a power:
   \[
   y = (4x^3 + 5x^2 - x + 6)^{\frac{1}{2}}
   \]

2. Identify the outer and inner functions:
   - Outer function: \( u(v) = v^{\frac{1}{2}} \), where \( v = 4x^3 + 5x^2 - x + 6 \).
   - Inner function: \( v(x) = 4x^3 + 5x^2 - x + 6 \).

3. Differentiate the outer function with respect to \( v \):
   \[
   \frac{du}{dv} = \frac{1}{2}v^{-\frac{1}{2}}
   \]

4. Differentiate the inner function with respect to \( x \):
   \[
   \frac{dv}{dx} = 12x^2 + 10x - 1
   \]

5. Multiply the derivatives:
   \[
   \frac{dy}{dx} = \frac{1}{2}(4x^3 + 5x^2 - x + 6)^{-\frac{1}{2}} \cdot (12x^2 + 10x - 1)
   \]

Thus, the derivative is:

\[
\frac{dy}{dx} = \frac{1}{2}(4x^3 + 5x^2 - x + 6)^{-\frac{1}{2}} (12x^2 + 10x - 1)
\]

</details>

---

#### Ex3.

Differentiate the following function using the Chain Rule:

\[
y = (x^3 - 2x + 1)^4
\]

<details>
  <summary>
    <strong id="solution-title">Solution</strong>
  </summary>

**Solution:**

1. Identify the outer and inner functions:
   - Outer function: \( u(v) = v^4 \), where \( v = x^3 - 2x + 1 \).
   - Inner function: \( v(x) = x^3 - 2x + 1 \).

2. Differentiate the outer function with respect to \( v \):
   \[
   \frac{du}{dv} = 4v^3
   \]

3. Differentiate the inner function with respect to \( x \):
   \[
   \frac{dv}{dx} = 3x^2 - 2
   \]

4. Multiply the derivatives:
   \[
   \frac{dy}{dx} = 4(x^3 - 2x + 1)^3 \cdot (3x^2 - 2)
   \]

Thus, the derivative is:

\[
\frac{dy}{dx} = 4(x^3 - 2x + 1)^3 (3x^2 - 2)
\]

</details>

---

#### Ex4.

Differentiate the following function using the Chain Rule:

\[
y = \frac{1}{\sqrt{5x^2 - 3x + 4}}
\]

<details>
  <summary>
    <strong id="solution-title">Solution</strong>
  </summary>

**Solution:**

1. Rewrite the function as a power:
   \[
   y = (5x^2 - 3x + 4)^{-\frac{1}{2}}
   \]

2. Identify the outer and inner functions:
   - Outer function: \( u(v) = v^{-\frac{1}{2}} \), where \( v = 5x^2 - 3x + 4 \).
   - Inner function: \( v(x) = 5x^2 - 3x + 4 \).

3. Differentiate the outer function with respect to \( v \):
   \[
   \frac{du}{dv} = -\frac{1}{2}v^{-\frac{3}{2}}
   \]

4. Differentiate the inner function with respect to \( x \):
   \[
   \frac{dv}{dx} = 10x - 3
   \]

5. Multiply the derivatives:
   \[
   \frac{dy}{dx} = -\frac{1}{2}(5x^2 - 3x + 4)^{-\frac{3}{2}} \cdot (10x - 3)
   \]

Thus, the derivative is:

\[
\frac{dy}{dx} = -\frac{1}{2}(5x^2 - 3x + 4)^{-\frac{3}{2}} (10x - 3)
\]

</details>

---


<iframe src="https://script.google.com/macros/s/AKfycbywwJperMbdU4IYLSn7M4wUDEgzU1Ph7c5bHo8j-_RFXgOb0b6IaE_cLnZ-86nGAjuO7Q/exec" width="100%" height="1000px" frameborder="0" marginheight="0" marginwidth="0">Loading...</iframe>

